List -> Dequeue

src/linear/adt/Dequeue.dfy
@@ -1,25 +1,70 @@
-trait List {
+include "../../../src/linear/implementation/DoublyLinkedListWithLast.dfy"
+include "../../../src/linear/interface/Dequeue.dfy"
+
+class Dequeue1 extends Dequeue {
+  var list: DoublyLinkedListWithLast;
+
   function Depth(): nat
     ensures Depth() > 0
+  {
+    2
+  }
+
+  function Repr0(): set<object>
+    reads this
+  {
+    {list}
+  }
+
+  function Repr1(): set<object>
+    reads this, Repr0()
+  {
+    Repr0() + {list.list}
+  }
+
+  function Repr2(): set<object>
+    reads this, Repr1()
+  {
+    Repr1() + list.Repr()
+  }
 
   function ReprFamily(n: nat): set<object>
     decreases n
     requires n <= Depth()
     ensures n > 0 ==> ReprFamily(n) >= ReprFamily(n-1)
     reads this, if n == 0 then {} else ReprFamily(n-1)
-
-  function Repr(): set<object>
-    reads this, ReprFamily(Depth()-1)
   {
-    ReprFamily(Depth())
+    if n == 0 then
+      Repr0()
+    else if n == 1 then
+      Repr1()
+    else if n == 2 then
+      Repr2()
+    else
+      assert false;
+      {}
   }
 
   predicate Valid()
     reads this, Repr()
+  {
+    list.Valid()
+  }
 
   function Model(): seq<int>
     reads this, Repr()
     requires Valid()
+  {
+    list.Model()
+  }
+
+  constructor()
+    ensures Valid()
+    ensures Model() == []
+    ensures fresh(Repr())
+  {
+    list := new DoublyLinkedListWithLast();
+  }
 
   method Front() returns (x: int)
     requires Valid()
@@ -27,6 +72,9 @@ trait List {
     ensures Valid()
     ensures Model() == old(Model())
     ensures x == Model()[0]
+  {
+    x := list.Front();
+  }
 
   method PushFront(x: int)
     modifies Repr()
@@ -35,6 +83,9 @@ trait List {
     ensures Model() == [x] + old(Model())
     ensures Repr() > old(Repr())
     ensures fresh(Repr() - old(Repr()))
+  {
+    list.PushFront(x);
+  }
 
   method PopFront() returns (x: int)
     modifies Repr()
@@ -43,6 +94,9 @@ trait List {
     ensures Valid()
     ensures [x] + Model() == old(Model())
     ensures Repr() < old(Repr())
+  {
+    x := list.PopFront();
+  }
 
   method Back() returns (x: int)
     requires Valid()
@@ -50,6 +104,9 @@ trait List {
     ensures Valid()
     ensures Model() == old(Model())
     ensures x == Model()[|Model()|-1]
+  {
+    x := list.Back();
+  }
 
   method PushBack(x: int)
     modifies Repr()
@@ -58,6 +115,9 @@ trait List {
     ensures Model() == old(Model()) + [x]
     ensures Repr() > old(Repr())
     ensures fresh(Repr() - old(Repr()))
+  {
+    list.PushBack(x);
+  }
 
   method PopBack() returns (x: int)
     modifies Repr()
@@ -66,4 +126,7 @@ trait List {
     ensures Valid()
     ensures Model() + [x] == old(Model())
     ensures Repr() < old(Repr())
+  {
+    x := list.PopBack();
+  }
 }
