src/linear/interface/Dequeue.dfy
@@ -1,70 +1,25 @@
-include "../../../src/linear/implementation/DoublyLinkedListWithLast.dfy"
-include "../../../src/linear/interface/List.dfy"
-
-class List1 extends List {
-  var list: DoublyLinkedListWithLast;
-
+trait Dequeue {
   function Depth(): nat
     ensures Depth() > 0
-  {
-    2
-  }
-
-  function Repr0(): set<object>
-    reads this
-  {
-    {list}
-  }
-
-  function Repr1(): set<object>
-    reads this, Repr0()
-  {
-    Repr0() + {list.list}
-  }
-
-  function Repr2(): set<object>
-    reads this, Repr1()
-  {
-    Repr1() + list.Repr()
-  }
 
   function ReprFamily(n: nat): set<object>
     decreases n
     requires n <= Depth()
     ensures n > 0 ==> ReprFamily(n) >= ReprFamily(n-1)
     reads this, if n == 0 then {} else ReprFamily(n-1)
+
+  function Repr(): set<object>
+    reads this, ReprFamily(Depth()-1)
   {
-    if n == 0 then
-      Repr0()
-    else if n == 1 then
-      Repr1()
-    else if n == 2 then
-      Repr2()
-    else
-      assert false;
-      {}
+    ReprFamily(Depth())
   }
 
   predicate Valid()
     reads this, Repr()
-  {
-    list.Valid()
-  }
 
   function Model(): seq<int>
     reads this, Repr()
     requires Valid()
-  {
-    list.Model()
-  }
-
-  constructor()
-    ensures Valid()
-    ensures Model() == []
-    ensures fresh(Repr())
-  {
-    list := new DoublyLinkedListWithLast();
-  }
 
   method Front() returns (x: int)
     requires Valid()
@@ -72,9 +27,6 @@ class List1 extends List {
     ensures Valid()
     ensures Model() == old(Model())
     ensures x == Model()[0]
-  {
-    x := list.Front();
-  }
 
   method PushFront(x: int)
     modifies Repr()
@@ -83,9 +35,6 @@ class List1 extends List {
     ensures Model() == [x] + old(Model())
     ensures Repr() > old(Repr())
     ensures fresh(Repr() - old(Repr()))
-  {
-    list.PushFront(x);
-  }
 
   method PopFront() returns (x: int)
     modifies Repr()
@@ -94,9 +43,6 @@ class List1 extends List {
     ensures Valid()
     ensures [x] + Model() == old(Model())
     ensures Repr() < old(Repr())
-  {
-    x := list.PopFront();
-  }
 
   method Back() returns (x: int)
     requires Valid()
@@ -104,9 +50,6 @@ class List1 extends List {
     ensures Valid()
     ensures Model() == old(Model())
     ensures x == Model()[|Model()|-1]
-  {
-    x := list.Back();
-  }
 
   method PushBack(x: int)
     modifies Repr()
@@ -115,9 +58,6 @@ class List1 extends List {
     ensures Model() == old(Model()) + [x]
     ensures Repr() > old(Repr())
     ensures fresh(Repr() - old(Repr()))
-  {
-    list.PushBack(x);
-  }
 
   method PopBack() returns (x: int)
     modifies Repr()
@@ -126,7 +66,4 @@ class List1 extends List {
     ensures Valid()
     ensures Model() + [x] == old(Model())
     ensures Repr() < old(Repr())
-  {
-    x := list.PopBack();
-  }
 }
